src/PlutusIR/Semantics/Static/Typing_sound_complete.v
@@ -1,0 +1,67 @@
+From PlutusCert Require Import 
+    Normalisation.Normalisation 
+    Strong_normalisation
+    Norm_sound_complete
+    Static.Typing 
+    PlutusIR 
+    Util.List
+    Static.Util.
+
+Fixpoint type_check (Γ : list (binderName * ty)) (term : term) : (option ty) :=
+    match term with
+    | Var x => lookup x Γ >>= fun T => normaliser_Jacco T
+    | LamAbs x T1 t => 
+        normaliser_Jacco T1 >>= fun T1n =>
+        match type_check ((x, T1n) :: Γ) t with
+        | Some T2 => Some (Ty_Fun T1n T2) (* TODO: no normalisation of T2? Is it always normal? In the has_type efinition it is called T2n, so maybe it is*)
+        | _ => None
+        end
+    (* | Apply t1 t2 =>
+        match type_check Γ t1, type_check Γ t2 with
+        | Some (Ty_Fun T1 T2), Some T1' =>
+            if eqb_ty T1 T1' then Some T2 else None
+        | (_, _) => None
+        end *)
+    | _ => None (* TODO *)
+    end. (* TODO: normalisation? *)
+
+
+
+
+    | Ty_Var X => (* Based on Software Foundations and has_kind *)
+        lookup X Delta
+    | Ty_Fun T1 T2 => (* TODO: I don't understand what this datatype does*)
+        match (kind_check Delta T1, kind_check Delta T2) with
+        | (Some Kind_Base, Some Kind_Base) => Some Kind_Base
+        | (_, _) => None
+        end
+    | Ty_IFix F T => (* Note: Purely based on structure of has_kind *)
+        match kind_check Delta T with
+        | Some K => match kind_check Delta F with
+            | Some (Kind_Arrow (Kind_Arrow K1 Kind_Base) (Kind_Arrow K2 Kind_Base)) =>
+                if andb (eqb_kind K K1) (eqb_kind K K2) then Some Kind_Base else None
+            | _ => None
+            end
+        | _ => None
+        end
+    | Ty_Forall X K T =>
+        match kind_check ((X, K) :: Delta) T with
+        | Some Kind_Base => Some Kind_Base
+        | _ => None
+        end
+    | Ty_Builtin d =>
+        kind_check_default_uni d
+    | Ty_Lam X K1 T => 
+        match kind_check ((X, K1) :: Delta) T with
+        | Some K2 => Some (Kind_Arrow K1 K2)
+        | _ => None
+        end
+    | Ty_App T1 T2 => 
+        match (kind_check Delta T1, kind_check Delta T2) with
+        | (Some (Kind_Arrow K11 K2), Some K12) =>
+            if eqb_kind K11 K12 then Some K2 else None
+        | (_, _) => None
+        end
+    end.
+
+
