src/PlutusIR/Semantics/Static/Util.v
@@ -1,0 +1,11 @@
+
+(* Monad maybe*)
+(* Define the bind function for option type *)
+Definition bind {A B : Type} (xx : option A) (f : A -> option B) : option B :=
+  match xx with
+  | None => None
+  | Some a => f a
+  end.
+
+(* Define an infix operator for bind *)
+Infix ">>=" := bind (at level 50, left associativity).
